High-level sketch for the requirements of a synthesizer.

src/Synthesis.v
@@ -1,21 +1,60 @@
 Require Import Bool List String Peano_dec.
-Require Import Common FMap Syntax Semantics Simulation.
+Require Import Common FMap Syntax Semantics SemFacts.
+Require Import StepDet StepSeq Serial SerialFacts Simulation.
 
-Section Synthesis.
+Section SimP.
 
-  (** Requirements *)
+  (** User inputs *)
   Variables
-    (stepI stepS: Step TState TLabel)
-    (impl0 spec: System) (* an initial system and the spec *)
+    (impl0 spec: System)
     (R: TState -> TState -> Prop)
-    (p: Label -> Label)
-    (Hrinit: R (getStateInit impl0) (getStateInit spec))
-    (Hsim: Simulates stepI stepS R p impl0 spec). (* a simulation relation *)
+    (p: Label -> Label).
+  
+  Definition SynthOk (s: System) :=
+    Serial s step_det /\
+    R (getStateInit s) (getStateInit spec) /\
+    Simulates step_seq step_det R p s spec.
 
-  Lemma impl0_ok: stepI # stepS |-- impl0 ⊑[p] spec.
-  Proof.
-    eapply simulation_implies_refinement; eauto.
-  Qed.
+  Hypothesis (Hinit_ok: SynthOk impl0).
 
-End Synthesis.
+  Section SynthesisStep.
+
+    Variable syn: System -> System -> Prop.
+    Infix "↪" := syn (at level 30).
+
+    (** The synthesizer [syn] should "preserve" three conditions:
+     * 1) initial state
+     * 2) serializability
+     * 3) simulation on sequential semantics
+     *)
+    Hypotheses (Hsyn_init: forall s s', syn s s' -> getStateInit s' = getStateInit s)
+               (Hsyn_serial:
+                  forall s, Serial s step_det ->
+                            forall s', syn s s' -> Serial s' step_det)
+               (Hsyn_sim:
+                  forall s, Simulates step_seq step_det R p s spec ->
+                            forall s', syn s s' ->
+                                       Simulates step_seq step_det R p s' spec).
+
+    Lemma synthOk_refinement:
+      forall s, SynthOk s -> step_det # step_det |-- s ⊑[p] spec.
+    Proof.
+      unfold SynthOk; intros; dest.
+      eapply refines_trans.
+      - apply sequential_step_seq.
+        eauto using Hsyn_serial.
+      - apply simulation_implies_refinement with (sim:= R); assumption.
+    Qed.
+
+    Lemma synthOk_preserved:
+      forall s s', SynthOk s -> syn s s' -> SynthOk s'.
+    Proof.
+      unfold SynthOk; intros; dest.
+      repeat split; eauto.
+      erewrite Hsyn_init; eauto.
+    Qed.
+
+  End SynthesisStep.
+
+End SimP.
 
